Weaker form of staged locks/invariants, proof of shadow ptr to show use.
This avoids the need for leases is the shadow pointer atomic pair proof, and
I think it makes it quite a bit simpler. It is also shorter:

     spec    proof comments
      119      154        2 RefinementShadowStaged.v
      142      198        9 RefinementShadow.v

(Some of the savings is because after making the change, it was clearer to me
how to shorten the simplified proof further).

This is not much longer than the POCS AtomicPair reference solution now.

src/CSL/StagedInvariant.v
@@ -8,98 +8,109 @@ Set Default Proof Using "Type".
 Import uPred.
 
 Class stagedG (Σ : gFunctors) : Set := WsatG {
-  staging_saved_inG :> savedPropG Σ;
-  staging_auth_inG :> inG Σ (authR (optionUR (exclR gnameC)));
+  staging_auth_inG :> inG Σ (authR (optionUR (exclR positiveC)));
 }.
 
-Definition staged_inv `{!invG Σ, !stagedG Σ} (N: namespace) (γ: gname) (Q: iProp Σ) : iProp Σ :=
-  (inv N (∃ γprop P, own γ (● Excl' γprop) ∗ saved_prop_own γprop P ∗ P ∗ □ (P -∗ Q)))%I.
+Definition stagedΣ : gFunctors := #[GFunctor (authR (optionUR (exclR positiveC)))].
+Instance subG_stagedΣ {Σ} : subG stagedΣ Σ → stagedG Σ.
+Proof. solve_inG. Qed.
 
-Definition staged_value `{!stagedG Σ} (N: namespace) (γ: gname) (Q: iProp Σ) : iProp Σ :=
-  (∃ γprop, own γ (◯ Excl' γprop) ∗ saved_prop_own γprop Q)%I.
+Definition staged_inv `{!invG Σ, !stagedG Σ} `{Countable A} (N: namespace) (γ: gname)
+           (Φ: A → iProp Σ) : iProp Σ :=
+  (inv N (∃ a, own γ (● Excl' (encode a)) ∗ Φ a))%I.
+
+Definition staged_value `{!stagedG Σ} `{Countable A} (N: namespace) γ (a: A)
+  : iProp Σ := own γ (◯ Excl' (encode a)).
 
 Section inv.
 Context `{!invG Σ, !stagedG Σ}.
+Context `{Countable A}.
 Implicit Types i : positive.
 Implicit Types N : namespace.
+Implicit Types Φ : A → iProp Σ.
 Implicit Types P Q R : iProp Σ.
 
+(* TODO *)
+(*
 Global Instance staged_contractive N γ : Contractive (staged_inv N γ).
 Proof. rewrite /staged_inv. solve_contractive. Qed.
+*)
 
-Global Instance staged_ne N γ : NonExpansive (staged_inv N γ).
-Proof. apply contractive_ne, _. Qed.
+Global Instance staged_ne N γ :
+  Proper (pointwise_relation A (dist n) ==> dist n) (staged_inv N γ).
+Proof. intros. solve_proper. Qed.
 
-Global Instance staged_proper N γ : Proper ((⊣⊢) ==> (⊣⊢)) (staged_inv N γ).
-Proof. apply ne_proper, _. Qed.
-
-Global Instance staged_persistent N γ P : Persistent (staged_inv N γ P).
-Proof. rewrite /staged_inv. apply _. Qed.
-
-Lemma staged_inv_iff N γ P Q : ▷ □ (P ↔ Q) -∗ staged_inv N γ P -∗ staged_inv N γ Q.
+Global Instance staged_proper N γ :
+  Proper (pointwise_relation A (⊣⊢) ==> (⊣⊢)) (staged_inv N γ).
 Proof.
-  iIntros "#HPQ". iApply inv_iff. iNext. iAlways. iSplit.
-  - iIntros "H". iDestruct "H" as (? P0) "(?&?&?&#HP0)". iExists _, P0. iFrame.
-    iAlways. iIntros. iApply "HPQ". by iApply "HP0".
-  - iIntros "H". iDestruct "H" as (? P0) "(?&?&?&#HP0)". iExists _, P0. iFrame.
-    iAlways. iIntros. iApply "HPQ". by iApply "HP0".
+  intros Φ1 Φ2 HΦ. apply equiv_dist=> n.
+  apply staged_ne=> x. apply equiv_dist, HΦ.
 Qed.
 
-Lemma staged_inv_alloc N E P Q: ▷ Q ∗ □ (Q -∗ P) ={E}=∗ ∃ γ, staged_inv N γ P ∗ staged_value N γ Q.
+Global Instance staged_persistent N γ (Φ : A → iProp Σ) : Persistent (staged_inv N γ Φ).
+Proof. rewrite /staged_inv. apply _. Qed.
+
+Lemma staged_inv_iff N γ Φ1 Φ2 :
+  ▷ □ (∀ x, Φ1 x ↔ Φ2 x) -∗ staged_inv N γ Φ1 -∗ staged_inv N γ Φ2.
 Proof.
-  iMod (saved_prop_alloc Q) as (γprop) "#Hsaved".
-  iMod (own_alloc (● (Excl' γprop) ⋅ ◯ (Excl' γprop))) as (γ) "[H1 H2]".
+  iIntros "#HPQ". iApply inv_iff. iNext. iAlways. iSplit.
+  - iIntros "H". iDestruct "H" as (?) "(?&?)". iExists _. iFrame.
+    by iApply "HPQ".
+  - iIntros "H". iDestruct "H" as (?) "(?&?)". iExists _. iFrame.
+    by iApply "HPQ".
+Qed.
+
+Lemma staged_inv_alloc N E Φ x:
+  ▷ (Φ x) ={E}=∗ ∃ γ, staged_inv N γ Φ ∗ staged_value N γ x.
+Proof.
+  iMod (own_alloc (● (Excl' (encode x)) ⋅ ◯ (Excl' (encode x)))) as (γ) "[H1 H2]".
   { apply auth_both_valid_2; [econstructor | reflexivity]. }
   iIntros "HP".
   iMod (inv_alloc N E _ with "[HP H1]") as "HI"; last first.
   { iModIntro. iExists γ. iSplitL "HI".
     - iApply "HI".
-    - iExists γprop. by iFrame.
+    - by iFrame.
   }
-  iNext. iExists γprop, Q. iFrame. auto.
+  iNext. iExists x. by iFrame.
 Qed.
 
-Lemma staged_inv_open E N γ P Q:
-  ↑N ⊆ E → staged_inv N γ P ∗ staged_value N γ Q
-           ={E,E∖↑N}=∗ ▷ ▷ Q ∗ (∀ Q', ▷ Q' ∗ □ (Q' -∗ P) ={E∖↑N,E}=∗ staged_value N γ Q').
+Lemma staged_inv_open `{Inhabited A} E N γ Φ x:
+  ↑N ⊆ E → staged_inv N γ Φ ∗ staged_value N γ x
+           ={E,E∖↑N}=∗ ▷ (Φ x) ∗ (∀ x', ▷ Φ x' ={E∖↑N,E}=∗ staged_value N γ x').
 Proof.
   iIntros (?) "(#Hinv&Hval)".
-  iDestruct "Hval" as (γprop) "(Hγ&#Hsaved)".
-  iInv N as (γprop' Qsaved) "H" "HC".
-  iDestruct "H" as "(>Hγ'&#Hsaved'&HQ0&#Himp)".
-  iDestruct (own_valid_2 with "Hγ' Hγ") as "#H".
-  iDestruct "H" as %[<-%Excl_included%leibniz_equiv _]%auth_both_valid.
-  iSplitL "HQ0".
-  - iModIntro. iNext. iDestruct (saved_prop_agree with "Hsaved Hsaved'") as "Hequiv".
-    iNext. by iRewrite "Hequiv".
-  - iModIntro. iIntros (Q'). iIntros "(HQ'&#HQ'impl)".
-    iMod (saved_prop_alloc Q') as (γprop_new) "#Hsaved_new".
-    iMod (own_update_2 _ _ _ (● Excl' γprop_new ⋅ ◯ Excl' γprop_new) with "Hγ' Hγ") as "[Hγ' Hγ]".
-    { by apply auth_update, option_local_update, exclusive_local_update. }
-    iMod ("HC" with "[HQ' Hγ']").
-    * iNext. iExists _, _. iFrame "#". iFrame.
-    * iModIntro. iExists _. by iFrame.
+  iInv N as "H" "HC".
+  iDestruct "H" as (a) "(>Hγ&HΦ)".
+  iDestruct (own_valid_2 with "Hγ Hval") as "#H".
+  iDestruct "H" as %[Henc%Excl_included%leibniz_equiv _]%auth_both_valid.
+  apply encode_inj in Henc; subst.
+  iFrame.
+  iModIntro. iIntros (a'). iIntros "HΦ'".
+  iMod (own_update_2 _ _ _ (● Excl' (encode a') ⋅ ◯ Excl' (encode a')) with "Hγ Hval") as "[Hγ' Hγ]".
+  { by apply auth_update, option_local_update, exclusive_local_update. }
+  iMod ("HC" with "[HΦ' Hγ']").
+  * iNext. iExists _. by iFrame.
+  * iModIntro. by iFrame.
 Qed.
 
-Lemma staged_inv_weak_open E N γ P:
-  ↑N ⊆ E → staged_inv N γ P ={E,E∖↑N}=∗ ▷ P.
+Lemma staged_inv_weak_open E N γ Φ:
+  ↑N ⊆ E → staged_inv N γ Φ ={E,E∖↑N}=∗ ▷ (∃ x, Φ x).
 Proof.
   iIntros (?) "#Hinv".
-  iInv N as (γprop' Qsaved) "H" "HC".
-  iDestruct "H" as "(>Hγ'&#Hsaved'&HQ0&#Himp)".
-  iModIntro. iNext. iApply "Himp". eauto.
+  iInv N as "H" "HC".
+  iModIntro. iNext. iDestruct "H" as (?) "(?&?)". iExists _. by iFrame.
 Qed.
 
-Global Instance into_inv_staged_inv1 N γ P : IntoInv (staged_inv N γ P) N := {}.
+Global Instance into_inv_staged_inv1 N γ Φ : IntoInv (staged_inv N γ Φ) N := {}.
 
-Definition staged_inv_exact N Pweak P :=
-  (∃ γ, staged_inv N γ Pweak ∗ staged_value N γ P)%I.
+Definition staged_inv_exact N Φ (x: A) :=
+  (∃ γ, staged_inv N γ Φ ∗ staged_value N γ x)%I.
 
 (*
-Global Instance into_acc_inv E N γ Pweak P :
-  IntoAcc (staged_inv_exact N γ Pweak P)
+Global Instance into_acc_inv E N Φ x :
+  IntoAcc (staged_inv_exact N Φ x)
           (↑N ⊆ E) True (fupd E (E∖↑N)) (fupd (E∖↑N) E)
-          (λ _, ▷ ▷ P)%I (λ Q, Q ∗ ▷ P)%I (λ Q, Some (staged_value N γ Q))%I.
+          (λ x, Φ x)%I (λ x, ▷ Φ x)%I (λ x, None)%I.
 Proof.
   rewrite /IntoAcc /accessor.
   iIntros (?) "(#Hinv&Hvalue) _". iMod (staged_inv_open with "[Hvalue]") as "($&?)"; first done.
